fix TODOs in pipeline, required FitsStack.stack_usage_correct

compiler/src/compiler/FitsStack.v
@@ -1,5 +1,6 @@
 Require Import Coq.ZArith.ZArith.
-Require Import coqutil.Map.Interface.
+Require Import coqutil.Map.Interface coqutil.Map.Properties coqutil.Decidable.
+Require Import coqutil.Tactics.destr.
 Require Import coqutil.Z.Lia.
 Require Import compiler.FlatImp.
 Require Import compiler.FlatToRiscvCommon.
@@ -7,6 +8,39 @@ Require Import compiler.FlatToRiscvFunctions.
 Require Import compiler.Simp.
 
 Local Open Scope Z_scope.
+
+Module map.
+  Lemma split_put_l2r{K V: Type}{map: map.map K V}{ok: map.ok map}
+        {keqb: K -> K -> bool}{keqb_spec: EqDecider keqb}:
+    forall m m1 m2 k v,
+      map.get m1 k = None ->
+      map.split m (map.put m1 k v) m2 ->
+      map.split m m1 (map.put m2 k v).
+  Proof.
+    unfold map.split, map.disjoint.
+    intros. simp. split.
+    - apply map.map_ext.
+      intros.
+      rewrite !map.get_putmany_dec.
+      rewrite !map.get_put_dec.
+      destr (keqb k k0).
+      + subst.
+        destr (map.get m2 k0). 2: reflexivity.
+        specialize H0r with (2 := E).
+        rewrite map.get_put_same in H0r.
+        exfalso. eauto.
+      + destr (map.get m2 k0); reflexivity.
+    - intros.
+      rewrite map.get_put_dec in H1.
+      destr (keqb k k0).
+      + subst.
+        simp.
+        congruence.
+      + specialize H0r with (2 := H1).
+        rewrite map.get_put_diff in H0r by congruence.
+        eauto.
+  Qed.
+End map.
 
 Section FitsStack.
   Context {p: FlatToRiscvCommon.parameters}.
@@ -44,26 +78,42 @@ Section FitsStack.
   Definition stack_usage_of_fun(funimpls: env)(f_entrypoint: String.string): option Z :=
     stack_usage_rec (S (count_funs funimpls)) funimpls (SCall nil f_entrypoint nil).
 
+  Definition update_stack_usage(e_glob: env)
+             (current: option Z)(fname: String.string)(fimpl: list Z * list Z * stmt Z): option Z :=
+    match current with
+    | Some cur => match fimpl with
+                  | (nil, nil, fbody) => match stack_usage_of_fun e_glob fname with
+                                         | Some res => Some (Z.max cur res)
+                                         | None => None
+                                         end
+                  | _ => Some cur
+                  end
+    | None => None
+    end.
+
   Definition stack_usage(funimpls: env): option Z :=
-    map.fold (fun res fname '(argnames, retnames, body) =>
-                match res with
-                | Some res => match argnames, retnames with
-                              | nil, nil => match stack_usage_of_fun funimpls fname with
-                                            | Some res' => Some (Z.max res res')
-                                            | None => None
-                                            end
-                              | _, _ => Some res
-                              end
-                | None => None
-                end)
-             (Some 0)
-             funimpls.
+    map.fold (update_stack_usage funimpls) (Some 0) funimpls.
 
   Lemma fits_stack_monotone: forall e z1 s,
       fits_stack z1 e s -> forall z2, z1 <= z2 -> fits_stack z2 e s.
   Proof.
     induction 1; intros; econstructor; eauto; try blia.
     eapply IHfits_stack. blia.
+  Qed.
+
+  Context {env_ok: map.ok env}.
+
+  Lemma fits_stack_monotone_env: forall e1 z s,
+      fits_stack z e1 s -> forall e2, map.extends e2 e1 -> fits_stack z e2 s.
+  Proof.
+    induction 1; intros; econstructor; eauto; try blia.
+    eapply IHfits_stack. (* TODO make map solver work: Solver.map_solver env_ok. *)
+    unfold map.extends in *.
+    intros.
+    rewrite map.get_remove_dec.
+    Tactics.destruct_one_match.
+    - subst. rewrite map.get_remove_same in H2. assumption.
+    - rewrite map.get_remove_diff in H2 by congruence. eauto.
   Qed.
 
   Lemma stack_usage_rec_correct: forall n e s z,
@@ -79,6 +129,82 @@ Section FitsStack.
       econstructor. 1: eassumption.
       eapply IHn. Fail rewrite E0. (* PARAMRECORDS *) etransitivity. 1: exact E0.
       f_equal. unfold framelength. blia.
+  Qed.
+
+  (* The art of figuring out the right induction hypothesis... *)
+  Let P(e_glob e_done: env)(r: option Z): Prop :=
+    forall e_rest f fbody z,
+      r = Some z ->
+      map.get e_done f = Some (nil, nil, fbody) ->
+      map.split e_glob e_done e_rest ->
+      fits_stack z e_glob fbody.
+
+  Lemma stack_usage_correct_aux: forall e_glob e_done,
+      P e_glob e_done (map.fold (update_stack_usage e_glob) (Some 0) e_done).
+  Proof.
+    intro e_glob. eapply map.fold_spec.
+    - subst P. cbv beta. intros. rewrite map.get_empty in H0. discriminate.
+    - intros. subst P. cbv beta in *.
+      intros.
+      destruct v as [ [ newargs newrets ] newbody ].
+      unfold update_stack_usage in *.
+      simp.
+      pose proof H3 as A.
+      apply map.split_put_l2r in A. 2: assumption.
+      destruct newargs; destruct newrets. {
+        unfold stack_usage_of_fun in *.
+        simpl in H1.
+        simp.
+        assert (map.get e_glob k = Some (nil, nil, newbody)) as Q. {
+          clear -H3 E0 H env_ok.
+          unfold map.split, map.disjoint in *.
+          simp.
+          etransitivity. 1: exact E0.
+          rewrite map.get_putmany_left in E0.
+          - rewrite map.get_put_same in E0. congruence.
+          - match goal with
+            | |- ?x = None => destr x
+            end.
+            2: reflexivity.
+            exfalso.
+            eapply H3r. 2: exact E.
+            rewrite map.get_put_same. reflexivity.
+        }
+        simpl in Q,E0. rewrite Q in E0. symmetry in E0. simp.
+        rewrite map.get_put_dec in H2.
+        eapply stack_usage_rec_correct in E1.
+        destr (String.eqb k f).
+        * simp. subst.
+          eapply fits_stack_monotone. {
+            eapply fits_stack_monotone_env. 1: eassumption.
+            unfold map.extends in *.
+            intros.
+            rewrite map.get_remove_dec in H1. simp.
+            assumption.
+          }
+          blia.
+        * specialize H0 with (1 := eq_refl).
+          eapply fits_stack_monotone.
+          -- eauto.
+          -- blia.
+      }
+      all: rewrite map.get_put_dec in H2.
+      all: destr (String.eqb k f); try discriminate.
+      all: simp; eauto.
+  Qed.
+
+  Lemma stack_usage_correct: forall e z f fbody,
+      map.get e f = Some (nil, nil, fbody) ->
+      stack_usage e = Some z ->
+      fits_stack z e fbody.
+  Proof.
+    intros. unfold stack_usage in *.
+    pose proof stack_usage_correct_aux as Q.
+    subst P.
+    cbv beta in Q.
+    eapply Q with (e_rest := map.empty); try eassumption.
+    apply map.split_empty_r.
+    reflexivity.
   Qed.
 
 End FitsStack.
